Proved minimization equality
-- Added proofs about Finset equality
-- Added minimization equality

lean4/Automaton/DFA/Minimization.lean
@@ -7,28 +7,28 @@ open DFA Finset
 
 namespace DFA
 
-variable {σ : Type _} {q : Type _} (r s t : DFA σ q) [DecidableEq σ] [DecidableEq q]
+variable {σ : Type _} {q : Type _} {r s t : DFA σ q} [DecidableEq σ] [DecidableEq q]
 
 @[simp]
-def minimization_reachable_q : Finset t.qs := t.qs.attach.filter (fun q => reachable t t.init q)
+def minimization_reachable_q (t : DFA σ q) : Finset t.qs := t.qs.attach.filter (fun q => reachable t t.init q)
 
 @[simp]
-def minimization_reachable_init : { x // x ∈ minimization_reachable_q t } := by
+def minimization_reachable_init (t : DFA σ q) : { x // x ∈ minimization_reachable_q t } := by
   exact ⟨t.init , by simp [finenum_to_finset]; exact reachable.base⟩
 
 @[simp]
-def minimization_reachable_fs : Finset {x // x ∈ minimization_reachable_q t} := by
+def minimization_reachable_fs (t : DFA σ q) : Finset {x // x ∈ minimization_reachable_q t} := by
   have := Finset.attach (minimization_reachable_q t)
   exact this.filter (fun q => q.1 ∈ t.fs)
 
 @[simp]
-def minimization_reachable_δ : { x // x ∈ minimization_reachable_q t } → t.σs → { x // x ∈ minimization_reachable_q t } := by
+def minimization_reachable_δ (t : DFA σ q) : { x // x ∈ minimization_reachable_q t } → t.σs → { x // x ∈ minimization_reachable_q t } := by
   intro q e
   have := q.2
   simp [finenum_to_finset] at this
   exact ⟨ t.δ q e, by simp [finenum_to_finset]; apply reachable.step; exact this⟩
 
-def minimization_reachable : DFA σ {x // x ∈ t.qs} :=
+def minimization_reachable (t : DFA σ q) : DFA σ {x // x ∈ t.qs} :=
   {qs := minimization_reachable_q t, init := minimization_reachable_init t, fs := minimization_reachable_fs t, δ := minimization_reachable_δ t}
 
 lemma minimization_reachable_δ_star'_eq (w : word t.σs) : (q : t.qs) → (r : reachable t t.init q) → δ_star' t q w = (δ_star' (minimization_reachable t) ⟨q, by simp [finenum_to_finset, minimization_reachable]; exact r⟩  w).1 := by
@@ -46,7 +46,7 @@ theorem minimization_reachable_δ_star_eq (w : word t.σs) : δ_star t w = (δ_s
   apply minimization_reachable_δ_star'_eq
   exact reachable.base
 
-theorem minimization_reachable_eq (w : word t.σs) : dfa_accepts t w ↔ dfa_accepts (minimization_reachable t) w := by
+theorem minimization_reachable_eq {w : word t.σs} : dfa_accepts t w ↔ dfa_accepts (minimization_reachable t) w := by
   apply Iff.intro
   · intro dfa
     simp only [dfa_accepts] at dfa
@@ -67,9 +67,9 @@ inductive distinct : t.qs → t.qs → Prop where
   | base (a b : t.qs) : ¬(a ∈ t.fs ↔ b ∈ t.fs) → distinct a b
   | step (a b : t.qs) : ∀ s : t.σs, distinct (t.δ a s) (t.δ b s) → distinct a b
 
-def nondistinct (a b : t.qs) : Prop := ¬ distinct t a b
+def nondistinct (a b : t.qs) : Prop := ¬ distinct a b
 
-lemma distinct_if_δ_star'_distinct (w : word t.σs) : (a b : t.qs) → distinct t (δ_star' t a w) (δ_star' t b w) → distinct t a b := by
+lemma distinct_if_δ_star'_distinct (w : word t.σs) : (a b : t.qs) → distinct (δ_star' t a w) (δ_star' t b w) → distinct a b := by
   induction w using List.reverseRecOn  with
   | H0 => intro a b d
           simp at d
@@ -81,7 +81,7 @@ lemma distinct_if_δ_star'_distinct (w : word t.σs) : (a b : t.qs) → distinct
                 exact d
 
 
-theorem distinct_iff_ex_notaccepted (a b : t.qs) : distinct t a b ↔ ∃ l : word t.σs, ¬(δ_star' t a l ∈ t.fs ↔ δ_star' t b l ∈ t.fs) := by
+theorem distinct_iff_ex_notaccepted (a b : t.qs) : distinct a b ↔ ∃ l : word t.σs, ¬(δ_star' t a l ∈ t.fs ↔ δ_star' t b l ∈ t.fs) := by
   apply Iff.intro
   · intro d
     induction d with
@@ -92,22 +92,22 @@ theorem distinct_iff_ex_notaccepted (a b : t.qs) : distinct t a b ↔ ∃ l : wo
   · intro ex
     apply Exists.elim ex
     intro c ex
-    have : distinct t (δ_star' t a c) (δ_star' t b c) := by apply distinct.base
-                                                            exact ex
+    have : distinct (δ_star' t a c) (δ_star' t b c) := by apply distinct.base
+                                                          exact ex
     apply distinct_if_δ_star'_distinct
     exact this
 
-lemma nondistinct_iff_nex_notaccepted : nondistinct t a b ↔ ¬∃ w : word t.σs, ¬(δ_star' t a w ∈ t.fs ↔ δ_star' t b w ∈ t.fs) := by
+lemma nondistinct_iff_nex_notaccepted : nondistinct a b ↔ ¬∃ w : word t.σs, ¬(δ_star' t a w ∈ t.fs ↔ δ_star' t b w ∈ t.fs) := by
   simp only [nondistinct]
   apply not_congr
   apply distinct_iff_ex_notaccepted
 
-theorem nondistinct_iff_forall_accepted : nondistinct t a b ↔ ∀ w : word t.σs, (δ_star' t a w ∈ t.fs ↔ δ_star' t b w ∈ t.fs) := by
+theorem nondistinct_iff_forall_accepted : nondistinct a b ↔ ∀ w : word t.σs, (δ_star' t a w ∈ t.fs ↔ δ_star' t b w ∈ t.fs) := by
   rw [←Decidable.not_exists_not]
   apply nondistinct_iff_nex_notaccepted
 
 
-theorem nondistinct.Symm {a b: t.qs} : nondistinct t a b → nondistinct t b a := by
+theorem nondistinct.Symm {a b: t.qs} : nondistinct a b → nondistinct b a := by
   intro n
   simp only [nondistinct]
   simp only [nondistinct] at n
@@ -126,7 +126,7 @@ theorem nondistinct.Symm {a b: t.qs} : nondistinct t a b → nondistinct t b a :
                       apply distinct.step
                       exact d
 
-theorem nondistinct.Refl {a : t.qs} : nondistinct t a a := by
+theorem nondistinct.Refl {a : t.qs} : nondistinct a a := by
   intro d
   rw [distinct_iff_ex_notaccepted] at d
   apply Exists.elim d
@@ -134,7 +134,7 @@ theorem nondistinct.Refl {a : t.qs} : nondistinct t a a := by
   apply h
   rfl
 
-theorem nondistinct.Trans {a b c : t.qs} : nondistinct t a b → nondistinct t b c → nondistinct t a c := by
+theorem nondistinct.Trans {a b c : t.qs} : nondistinct a b → nondistinct b c → nondistinct a c := by
   intro n₁ n₂
   rw [nondistinct_iff_forall_accepted] at n₁
   rw [nondistinct_iff_forall_accepted] at n₂
@@ -150,77 +150,93 @@ theorem nondistinct.Trans {a b c : t.qs} : nondistinct t a b → nondistinct t b
     apply (n₂ w).mpr
     exact cin
 
-instance instNondistinctEquivalence : Equivalence (nondistinct t) := by
+theorem nondistinct_step {a b : t.qs} {e : t.σs} : nondistinct a b → nondistinct (t.δ a e) (t.δ b e) := by
+  intro n
+  intro d
+  apply n
+  apply distinct.step
+  exact d
+
+theorem nondistinct_self {a : t.qs} : nondistinct a a := by
+  simp only [nondistinct]
+  intro d
+  rw [distinct_iff_ex_notaccepted] at d
+  apply Exists.elim d
+  intro l h
+  apply h
+  trivial
+
+instance instNondistinctEquivalence : Equivalence (@nondistinct σ q t) := by
   apply Equivalence.mk
-  · intro a; exact nondistinct.Refl t
-  · exact nondistinct.Symm t
-  · exact nondistinct.Trans t
+  · intro a; exact nondistinct.Refl
+  · exact nondistinct.Symm
+  · exact nondistinct.Trans
 
 -- Table filling algorithm
 
-def all_pairs : Finset (t.qs × t.qs) := t.qs.attach.biUnion (fun q₁ => t.qs.attach.biUnion (fun q₂ => {⟨q₁,q₂⟩}))
+def all_pairs (t : DFA σ q) : Finset (t.qs × t.qs) := t.qs.attach.biUnion (fun q₁ => t.qs.attach.biUnion (fun q₂ => {⟨q₁,q₂⟩}))
 
 def start : Finset (t.qs × t.qs) := (all_pairs t).filter (fun (a,b) => ¬(a ∈ t.fs ↔ b ∈ t.fs))
 
-lemma start_subset_all : (start t) ⊆ (all_pairs t) := by
+lemma start_subset_all : start  ⊆ all_pairs t := by
   simp [start]
 
 def step (c a : Finset (t.qs × t.qs)) : Finset (t.qs × t.qs) := c ∪ (a.filter (fun (a,b) => ∃ s : t.σs, (t.δ a s, t.δ b s) ∈ c))
 
-theorem table_aux_decreasing : ¬card (step t c (all_pairs t)) = card c → c ⊆ all_pairs t → (all_pairs t).card - (step t c (all_pairs t)).card < (all_pairs t).card - c.card := by
+theorem table_aux_decreasing : ¬card (step c (all_pairs t)) = card c → c ⊆ all_pairs t → (all_pairs t).card - (step c (all_pairs t)).card < (all_pairs t).card - c.card := by
   intro g h
-  have h₁ : (step t c (all_pairs t)).card >= c.card := by simp only [step]
-                                                          apply Finset.card_le_of_subset
-                                                          apply Finset.subset_union_left
-  have h₂ : card c < card (step t c (all_pairs t)) := by apply Nat.lt_iff_le_and_ne.mpr
-                                                         apply And.intro
-                                                         · exact h₁
-                                                         · simp at g
-                                                           intro eq
-                                                           apply g
-                                                           simp at eq
-                                                           apply Eq.symm
-                                                           exact eq
-  have s : step t c (all_pairs t) ⊆ (all_pairs t) := by simp only [step]
-                                                        apply Finset.union_subset
-                                                        · exact h
-                                                        · apply Finset.filter_subset
-  have d : c ⊂ step t c (all_pairs t) := by apply Finset.ssubset_iff_subset_ne.mpr
-                                            apply And.intro
-                                            · simp only [step]
-                                              apply Finset.subset_union_left
-                                            · intro eq
-                                              apply g
-                                              rw [←eq]
-  have : (all_pairs t).card - (step t c (all_pairs t)).card < (all_pairs t).card - c.card := by apply Nat.sub_lt_sub_left
-                                                                                                · apply Nat.lt_iff_le_and_ne.mpr
-                                                                                                  apply And.intro
-                                                                                                  · apply Finset.card_le_of_subset
-                                                                                                    exact h
-                                                                                                  · apply Nat.ne_of_lt
-                                                                                                    apply Finset.card_lt_card
-                                                                                                    apply Finset.ssubset_of_ssubset_of_subset
-                                                                                                    · exact d
-                                                                                                    · exact s
-                                                                                                · exact h₂
+  have h₁ : (step c (all_pairs t)).card >= c.card := by simp only [step]
+                                                        apply Finset.card_le_of_subset
+                                                        apply Finset.subset_union_left
+  have h₂ : card c < card (step c (all_pairs t)) := by apply Nat.lt_iff_le_and_ne.mpr
+                                                       apply And.intro
+                                                       · exact h₁
+                                                       · simp at g
+                                                         intro eq
+                                                         apply g
+                                                         simp at eq
+                                                         apply Eq.symm
+                                                         exact eq
+  have s : step c (all_pairs t) ⊆ (all_pairs t) := by simp only [step]
+                                                      apply Finset.union_subset
+                                                      · exact h
+                                                      · apply Finset.filter_subset
+  have d : c ⊂ step c (all_pairs t) := by apply Finset.ssubset_iff_subset_ne.mpr
+                                          apply And.intro
+                                          · simp only [step]
+                                            apply Finset.subset_union_left
+                                          · intro eq
+                                            apply g
+                                            rw [←eq]
+  have : (all_pairs t).card - (step c (all_pairs t)).card < (all_pairs t).card - c.card := by apply Nat.sub_lt_sub_left
+                                                                                              · apply Nat.lt_iff_le_and_ne.mpr
+                                                                                                apply And.intro
+                                                                                                · apply Finset.card_le_of_subset
+                                                                                                  exact h
+                                                                                                · apply Nat.ne_of_lt
+                                                                                                  apply Finset.card_lt_card
+                                                                                                  apply Finset.ssubset_of_ssubset_of_subset
+                                                                                                  · exact d
+                                                                                                  · exact s
+                                                                                              · exact h₂
   exact this
 
 def table_aux (c : Finset (t.qs × t.qs)) (h : c ⊆ (all_pairs t)) : Finset (t.qs × t.qs) := by
   let a := all_pairs t
-  if (step t c a).card = c.card then exact c else exact table_aux (step t c a) (by simp only [step]
-                                                                                   apply Finset.union_subset_iff.mpr
-                                                                                   apply And.intro
-                                                                                   · exact h
-                                                                                   · simp)
+  if (step c a).card = c.card then exact c else exact table_aux (step c a) (by simp only [step]
+                                                                               apply Finset.union_subset_iff.mpr
+                                                                               apply And.intro
+                                                                               · exact h
+                                                                               · simp)
 termination_by table_aux c h => (all_pairs t).card - c.card
-decreasing_by have : (all_pairs t).card - (step t c (all_pairs t)).card < (all_pairs t).card - c.card := by apply table_aux_decreasing t (by assumption) (by assumption)
+decreasing_by have : (all_pairs t).card - (step c (all_pairs t)).card < (all_pairs t).card - c.card := by apply table_aux_decreasing (by assumption) (by assumption)
               apply this
 
-def table_filling : Finset (t.qs × t.qs) := table_aux t (start t) (start_subset_all t)
+def table_filling : Finset (t.qs × t.qs) := table_aux start start_subset_all
 
-def distinct_table_filling (a b : t.qs) : Bool := ⟨a,b⟩ ∈ table_filling t
+def distinct_table_filling (a b : t.qs) : Bool := ⟨a,b⟩ ∈ table_filling
 
-lemma step_subset (a b : Finset _) : a ⊆ b → step t a b ⊆ b := by
+lemma step_subset (a b : Finset ({ x // x ∈ t.qs } × { x // x ∈ t.qs })) : a ⊆ b → step a b ⊆ b := by
   intro ss
   simp only [step]
   apply Finset.union_subset_iff.mpr
@@ -228,10 +244,10 @@ lemma step_subset (a b : Finset _) : a ⊆ b → step t a b ⊆ b := by
   · exact ss
   · simp
 
-lemma table_aux_eq_table_aux : table_aux t c h = if (step t c (all_pairs t)).card = c.card then c else table_aux t (step t c (all_pairs t)) (step_subset t c (all_pairs t) h) := by
+lemma table_aux_eq_table_aux : table_aux c h = if (step c (all_pairs t)).card = c.card then c else table_aux (step c (all_pairs t)) (step_subset c (all_pairs t) h) := by
   apply WellFounded.fixFEq
 
-theorem table_aux_forall (P : Finset (t.qs × t.qs) → Prop) (c : Finset (t.qs × t.qs)) {h : c ⊆ all_pairs t} : P c → (∀ f : Finset (t.qs × t.qs), P f → P (step t f (all_pairs t))) → P (table_aux t c h) := by
+theorem table_aux_forall (P : Finset (t.qs × t.qs) → Prop) (c : Finset (t.qs × t.qs)) {h : c ⊆ all_pairs t} : P c → (∀ f : Finset (t.qs × t.qs), P f → P (step f (all_pairs t))) → P (table_aux c h) := by
   intro b fa
   rw [table_aux_eq_table_aux]
   split
@@ -241,12 +257,12 @@ theorem table_aux_forall (P : Finset (t.qs × t.qs) → Prop) (c : Finset (t.qs 
       exact b
     · apply fa
 termination_by table_aux_forall p => (all_pairs t).card - c.card
-decreasing_by have : (all_pairs t).card - (step t c (all_pairs t)).card < (all_pairs t).card - c.card := by apply table_aux_decreasing t (by assumption) (by assumption)
+decreasing_by have : (all_pairs t).card - (step c (all_pairs t)).card < (all_pairs t).card - c.card := by apply table_aux_decreasing (by assumption) (by assumption)
               apply this
 
 def ex_word_prop : Finset (t.qs × t.qs) → Prop := fun f => ∀ p : (t.qs × t.qs), p ∈ f → ∃ w : word t.σs, ¬(δ_star' t p.1 w ∈ t.fs ↔ δ_star' t p.2 w ∈ t.fs)
 
-lemma exists_notaccepted_if_table_filling : ex_word_prop t (table_aux t (start t) (start_subset_all t)) := by
+lemma exists_notaccepted_if_table_filling (t : DFA σ q) : ex_word_prop (table_aux start (@start_subset_all σ q t _)) := by
   apply table_aux_forall
   · simp [ex_word_prop,start]
     intro a b c d _ nin
@@ -269,7 +285,7 @@ lemma exists_notaccepted_if_table_filling : ex_word_prop t (table_aux t (start t
                apply distinct.step
                exact this
 
-lemma step_gt_if (c : Finset _)(a b : t.qs) (e : t.σs): ⟨t.δ a e, t.δ b e⟩ ∈ c → ⟨a,b⟩ ∉ c → (step t c (all_pairs t)).card > c.card := by
+lemma step_gt_if (c : Finset _)(a b : t.qs) (e : t.σs): ⟨t.δ a e, t.δ b e⟩ ∈ c → ⟨a,b⟩ ∉ c → (step c (all_pairs t)).card > c.card := by
   intro inc ninc
   simp only [step]
   apply Finset.card_lt_card
@@ -285,7 +301,7 @@ lemma step_gt_if (c : Finset _)(a b : t.qs) (e : t.σs): ⟨t.δ a e, t.δ b e�
       · exists e
     · exact ninc
 
-lemma if_δ_in_table_aux_in_table_aux : ⟨t.δ a e, t.δ b e⟩ ∈ table_aux t c h → ⟨a,b⟩ ∈ table_aux t c h := by
+lemma if_δ_in_table_aux_in_table_aux : ⟨t.δ a e, t.δ b e⟩ ∈ table_aux c h → ⟨a,b⟩ ∈ table_aux c h := by
   intro δ
   rw [table_aux_eq_table_aux]
   rw [table_aux_eq_table_aux] at δ
@@ -293,9 +309,9 @@ lemma if_δ_in_table_aux_in_table_aux : ⟨t.δ a e, t.δ b e⟩ ∈ table_aux t
   · split at δ
     · cases (Decidable.em (⟨a,b⟩ ∈ c)) with
       | inl h => exact h
-      | inr h => have := step_gt_if t c a b e δ h
-                 have : card (step t c (all_pairs t)) ≠ card c := by apply Nat.ne_of_gt
-                                                                     exact this
+      | inr h => have := step_gt_if c a b e δ h
+                 have : card (step c (all_pairs t)) ≠ card c := by apply Nat.ne_of_gt
+                                                                   exact this
                  contradiction
     · contradiction
   · split at δ
@@ -303,36 +319,36 @@ lemma if_δ_in_table_aux_in_table_aux : ⟨t.δ a e, t.δ b e⟩ ∈ table_aux t
     · apply if_δ_in_table_aux_in_table_aux
       · exact δ
 termination_by if_δ_in_table_aux_in_table_aux p => (all_pairs t).card - c.card
-decreasing_by have : (all_pairs t).card - (step t c (all_pairs t)).card < (all_pairs t).card - c.card := by apply table_aux_decreasing t (by assumption) (by assumption)
+decreasing_by have : (all_pairs t).card - (step c (all_pairs t)).card < (all_pairs t).card - c.card := by apply table_aux_decreasing (by assumption) (by assumption)
               apply this
 
 
-lemma table_filling_if_exists (w : word t.σs): (a b : t.qs) → ¬(δ_star' t a w ∈ t.fs ↔ δ_star' t b w ∈ t.fs) → distinct_table_filling t a b := by
+lemma table_filling_if_exists (w : word t.σs): (a b : t.qs) → ¬(δ_star' t a w ∈ t.fs ↔ δ_star' t b w ∈ t.fs) → distinct_table_filling a b := by
   simp only [distinct_table_filling,table_filling]
   induction w  with
   | nil => intro a b h
-           simp at h
+           simp only [δ_star'] at h
            rw [decide_eq_true_eq]
            apply table_aux_forall
-           · simp [start]
-             simp at h
+           · simp only [start]
+             rw [Finset.mem_filter]
              apply And.intro
              · simp [all_pairs]
              · exact h
            · intro f inf
-             simp [step]
+             simp only [step]
+             apply Finset.mem_union.mpr
              apply Or.inl
              exact inf
     | cons e es s => intro a b h
                      rw [decide_eq_true_eq]
-                     simp at h
+                     simp only [δ_star] at h
                      have δ := s (t.δ a e) (t.δ b e) h
                      rw [decide_eq_true_eq] at δ
                      apply if_δ_in_table_aux_in_table_aux
                      exact δ
 
-
-theorem forall_step_exists_word (a b : t.qs) : distinct_table_filling t a b ↔ ∃ w : word t.σs, ¬(δ_star' t a w ∈ t.fs ↔ δ_star' t b w ∈ t.fs) := by
+theorem forall_step_exists_word (a b : t.qs) : distinct_table_filling a b ↔ ∃ w : word t.σs, ¬(δ_star' t a w ∈ t.fs ↔ δ_star' t b w ∈ t.fs) := by
   apply Iff.intro
   · intro d
     simp only [distinct_table_filling] at d
@@ -348,12 +364,153 @@ theorem forall_step_exists_word (a b : t.qs) : distinct_table_filling t a b ↔ 
     apply table_filling_if_exists
     . exact h
 
-
 instance instDecExW : Decidable (∃ w : word t.σs, ¬(δ_star' t a w ∈ t.fs ↔ δ_star' t b w ∈ t.fs)) := by
-  apply decidable_of_iff (distinct_table_filling t a b)
-  exact forall_step_exists_word t a b
+  apply decidable_of_iff (distinct_table_filling a b)
+  exact forall_step_exists_word a b
 
-instance instDecDistinct : Decidable (distinct t a b) := by
+instance instDecDistinct : Decidable (@distinct σ q t a b) := by
   apply decidable_of_iff (∃ w : word t.σs, ¬(δ_star' t a w ∈ t.fs ↔ δ_star' t b w ∈ t.fs))
   apply Iff.symm
   apply distinct_iff_ex_notaccepted
+
+instance instDecNondistinct : Decidable (@nondistinct σ q t a b) := by
+  simp only [nondistinct]
+  infer_instance
+
+-- Minimization of DFA using nondistinct states
+
+def min_q (t : DFA σ q) : Finset (Finset t.qs) := t.qs.attach.biUnion (fun q => {t.qs.attach.filter (fun q' => nondistinct q' q)})
+
+def min_init (t : DFA σ q) : { x // x ∈ min_q t } := by
+  simp only [min_q]
+  exact ⟨t.qs.attach.filter (fun q => nondistinct q t.init), by rw [Finset.mem_biUnion]; exists t.init; rw [Finset.mem_singleton]; exact ⟨by simp, rfl⟩⟩
+
+def min_fs (t : DFA σ q) : Finset { x // x ∈ min_q t } := (min_q t).attach.filter (fun f => ∃ q : t.qs, q ∈ f.1 ∧ q ∈ t.fs)
+
+theorem min_δ_step_in (a : { x // x ∈ min_q t }) : a.1.biUnion (fun a => (t.qs.attach).filter (fun b => nondistinct b (t.δ a e))) ∈ min_q t := by
+  simp only [min_q]
+  simp only [min_q] at a
+  have := a.2
+  simp at this
+  apply Exists.elim this
+  intro q ex
+  apply Exists.elim ex
+  intro b h
+  simp at h
+  rw [h]
+  rw [Finset.mem_biUnion]
+  exists (t.δ ⟨q,b⟩ e)
+  exists (by simp)
+  rw [Finset.mem_singleton]
+  apply mem_iff_mem_eq
+  intro el
+  rw [Finset.mem_biUnion,Finset.mem_filter]
+  apply Iff.intro
+  · intro elin
+    apply Exists.elim elin
+    intro q₁ h
+    rw [Finset.mem_filter,Finset.mem_filter] at h
+    have : nondistinct (t.δ q₁ e) (t.δ ⟨q,b⟩ e) := nondistinct_step h.1.2
+    apply And.intro
+    · simp
+    · apply nondistinct.Trans
+      exact h.2.2
+      exact this
+  · intro elin
+    exists ⟨q,b⟩
+    rw [Finset.mem_filter,Finset.mem_filter]
+    apply And.intro
+    · exact ⟨by simp, by apply nondistinct_self⟩
+    · exact ⟨by simp, by exact elin.2⟩
+
+
+def min_δ : { x // x ∈ min_q t } → { x // x ∈ t.σs } → { x // x ∈ min_q t } := by
+  intro a e
+  let b := a.1.biUnion (fun a => (t.qs.attach).filter (fun b => nondistinct b (t.δ a e)))
+  exact ⟨b , min_δ_step_in a⟩
+
+def min_dfa (t : DFA σ q) : DFA σ (Finset t.qs) := {qs := min_q t, σs := t.σs, init := min_init t, fs := min_fs t, δ := min_δ}
+
+def state_eq_class (a : t.qs) : { x // x ∈ (min_dfa t).qs } := ⟨t.qs.attach.filter (fun q => nondistinct q a), by simp [min_dfa,min_q]; exists a; exists (by simp)⟩
+
+lemma step_eq_class_eq : state_eq_class (DFA.δ t a e) = DFA.δ (min_dfa t) (state_eq_class a) e := by
+  simp [state_eq_class,min_dfa,min_δ]
+  apply mem_iff_mem_eq
+  intro q
+  apply Iff.intro
+  · intro ein
+    rw [Finset.mem_filter] at ein
+    rw [Finset.mem_biUnion]
+    simp
+    simp at ein
+    exists a
+    exists (by simp)
+    apply And.intro
+    · apply nondistinct_self
+    · exact ein
+  · intro ein
+    simp at ein
+    simp
+    apply Exists.elim ein
+    intro a₁ ex₁
+    apply Exists.elim ex₁
+    intro b₁ h
+    simp at h
+    apply nondistinct.Trans
+    · exact h.2
+    apply nondistinct_step
+    exact h.1
+
+theorem min_δ'_accepts_iff {w : word t.σs} : {a : t.qs} → (δ_star' t a w ∈ t.fs ↔ δ_star' (min_dfa t) (state_eq_class a) w ∈ (min_dfa t).fs) := by
+  induction w with
+  | nil => intro a
+           simp only [δ_star',state_eq_class,min_dfa]
+           apply Iff.intro
+           · intro ain
+             simp [min_fs]
+             apply And.intro
+             · simp [min_q]
+               apply Finset.mem_attach
+             · exists a
+               exists (by simp)
+               exact ⟨nondistinct_self, ain⟩
+           · intro h
+             simp [min_fs] at h
+             apply Exists.elim h.2
+             intro q ex
+             apply Exists.elim ex
+             intro p h
+             have := nondistinct_iff_forall_accepted.mp h.1 []
+             simp only [δ_star'] at this
+             apply this.mp
+             exact h.2
+  | cons e es s => intro a
+                   simp only [δ_star']
+                   have eq : state_eq_class (DFA.δ t a e) = DFA.δ (min_dfa t) (state_eq_class a) e := by apply step_eq_class_eq
+                   apply Iff.intro
+                   · intro din
+                     have s := s.mp din
+                     rw [←eq]
+                     exact s
+                   · intro sin
+                     rw [←eq] at sin
+                     have s := s.mpr sin
+                     exact s
+
+theorem min_eq {w : word t.σs} : dfa_accepts t w ↔ dfa_accepts (min_dfa t) w := by
+  simp only [dfa_accepts,δ_star]
+  apply min_δ'_accepts_iff
+
+theorem min_reachable_min_eq {w : word t.σs} : dfa_accepts (minimization_reachable t) w ↔ dfa_accepts (min_dfa (minimization_reachable t)) w := by
+  apply min_eq
+
+theorem min_min_eq {w : word t.σs} : dfa_accepts t w ↔ dfa_accepts (min_dfa (minimization_reachable t)) w := by
+  apply Iff.intro
+  · intro d
+    apply min_reachable_min_eq.mp
+    apply minimization_reachable_eq.mp
+    exact d
+  · intro d
+    apply minimization_reachable_eq.mpr
+    apply min_reachable_min_eq.mpr
+    exact d
